proof/invariant-abstract/ARM/ArchCSpace_AI.thy
@@ -575,6 +575,7 @@ crunches arch_post_cap_deletion
   and irq_node[wp]: "\<lambda>s. P (interrupt_irq_node s)"
   and invs_no_pre[wp]: invs
   and cur_thread[wp]:  "\<lambda>s. P (cur_thread s)"
+  and release_queue[wp]:  "\<lambda>s. P (release_queue s)"
   and state_refs_of[wp]: "\<lambda>s. P (state_refs_of s)"
   and mdb_inv[wp]: "\<lambda>s. P (cdt s)"
   and valid_list[wp]: valid_list
