proof/invariant-abstract/ARM/ArchSyscall_AI.thy
@@ -99,6 +99,7 @@ lemma hh_invs[wp, Syscall_AI_assms]:
 
 crunches make_fault_msg
   for cur_thread[wp, Syscall_AI_assms]: "\<lambda>s. P (cur_thread s)"
+  and cur_sc[wp, Syscall_AI_assms]: "\<lambda>s. P (cur_sc s)"
   and pred_tcb_at[wp, Syscall_AI_assms]: "pred_tcb_at proj P t"
 
 end
